Specialize detTraceIter into sliceIter

go/iterator/slice_iter.go
@@ -1,9 +1,9 @@
 package iterator
 
-func sliceIter[V any](s []V) func(yield func(V) bool) {
-	return func(yield func(V) bool) {
-		for _, v := range s {
-			if !yield(v) {
+func sliceIter[V any](s []V) func(yield func(int, V) bool) {
+	return func(yield func(int, V) bool) {
+		for i, v := range s {
+			if !yield(i, v) {
 				return
 			}
 		}
@@ -13,7 +13,8 @@ func sliceIter[V any](s []V) func(yield func(V) bool) {
 func isAscii(str []byte) bool {
 	ret_val := true
 
-	loop_body := func (b byte) bool {
+	loop_body := func (i int, b byte) bool {
+		_ = i
 		if (b >= 0x80 || b == 0x00) {
 			ret_val = false
 			return false
@@ -28,25 +29,4 @@ func isAscii(str []byte) bool {
 	iterator(loop_body)
 
 	return ret_val
-}
-
-func sliceIter2[V any](s []V) func(yield func(int, V) bool) {
-	return func(yield func(int, V) bool) {
-		for i, v := range s {
-			if !yield(i, v) {
-				return
-			}
-		}
-	}
-}
-
-// 0 indexed
-func euler_triangle_row(row int) []int {
-	s := make([]int, row + 1)
-
-	loop_body := func(i int, v int) bool {
-		if ()
-
-		return true
-	}
 }
